making V sv fsv parameters; mall_sound

ll/ll_semnd.v
@@ -142,26 +142,35 @@ Lemma bang_sem_mono (X X' : M -> Prop) :
   (forall u, X u -> X' u) -> (forall u, bang_sem X u -> bang_sem X' u).
 Proof. intros xx. apply dd_mono. firstorder. Qed.
 
-Fixpoint sem {V : Set} (sv : V -> M -> Prop) f := match f with 
+Variable V : Set.
+Variable sv : V -> M -> Prop. (* semantics of variables *)
+
+Fixpoint sem f := match f with 
   | Var v => sv v
   | DVar v => dual_sem (sv v)
   | Bot _ => bot
   | One _ => dual_sem (dual_sem (eq e))
   | Zero _ => dual_sem (dual_sem (fun _ => empty))
   | Top _ => fun _ => True
-  | tens A B => tens_sem (sem sv A) (sem sv B)
-  | par A B => par_sem (sem sv A) (sem sv B) 
-  | plus A B => dual_sem (dual_sem (fun x => sem sv A x \/ sem sv B x))
-  | wth A B => (fun x => sem sv A x /\ sem sv B x) 
-  | Bang f => bang_sem (sem sv f)
-  | Query f => query_sem (sem sv f)
+  | tens A B => tens_sem (sem A) (sem B)
+  | par A B => par_sem (sem A) (sem B) 
+  | plus A B => dual_sem (dual_sem (fun x => sem A x \/ sem B x))
+  | wth A B => (fun x => sem A x /\ sem B x) 
+  | Bang f => bang_sem (sem f)
+  | Query f => query_sem (sem f)
   end.
 
+Print Implicit sem.
+
 (* semantics of list of formula is sem of their par *)
-Definition seml {V} sv fs := fold_right par_sem bot (map (@sem V sv) fs).
+Definition seml fs := fold_right par_sem bot (map sem fs).
 (* note useful lemmas
   fold_left_rev_right fold_right_app fold_symmetric fold_left_app,
   need to prove more using assoc and comm and identity of par_sem *)
+
+Lemma seml_alt fs : seml fs = sem (fold_right (@par V) (@Bot V) fs).
+Proof. induction fs. reflexivity.
+unfold seml. simpl. apply f_equal. exact IHfs. Qed.
 
 (* fact and factd are equivalent *)
 Definition fact X := forall u, dual_sem (dual_sem X) u -> X u.
@@ -301,11 +310,16 @@ Lemma fact_bot : fact bot.
 Proof. unfold fact. intro.  rewrite - dual_sem_1.
 apply dual_anti. intros v ev. subst v. exact dual_sem_bot. Qed.
 
+Hypothesis fsv : forall v, fact (sv v).
+
 (* semantics of all formula interpretations are facts *)
-Lemma fact_sem {V} A sv : (forall v, fact (sv v)) -> fact (@sem V sv A).
-Proof. intros fv.  induction A ; simpl ; try (apply fact_dual).
-apply fv. apply fact_bot.  unfold fact. tauto.
+Lemma fact_sem A : fact (sem A).
+Proof.  induction A ; simpl ; try (apply fact_dual).
+apply fsv. apply fact_bot.  unfold fact. tauto.
 exact (facts_int IHA1 IHA2). Qed.
+
+Lemma fact_seml As : fact (seml As).
+Proof. rewrite seml_alt. apply fact_sem. Qed.
 
 Lemma dual_sem_or X Y v : 
   dual_sem (fun u => X u \/ Y u) v <-> dual_sem X v /\ dual_sem Y v.
@@ -314,8 +328,7 @@ firstorder.  firstorder.  firstorder. Qed.
 
 Lemma dual_sem_or' X Y : 
   dual_sem (fun u => X u \/ Y u) = (fun v => dual_sem X v /\ dual_sem Y v).
-Proof. apply FunctionalExtensionality.functional_extensionality.
-intro x.  apply ax_prop_ext.  apply dual_sem_or. Qed.
+Proof. apply iff_app_eq.  intro x.  apply dual_sem_or. Qed.
 
 Lemma dsao k A z : fact k -> dual_sem 
   (fun x => dual_sem A x /\ k x) z ->
@@ -488,10 +501,16 @@ Lemma tens_assocr X Y Z u :
 Proof. pose (@dual_anti _ _ (@tens_assocr_lem X Y Z) u).
 rewrite -> !(fact_dd_eq (@fact_tens _ _)) in d. exact d. Qed.
 
+Print Implicit fact_seml.
+
 Lemma par_assoc X Y Z u : 
   (par_sem X (par_sem Y Z)) u -> (par_sem (par_sem X Y) Z) u.
 Proof. unfold par_sem.  rewrite  !(fact_dd_eq (@fact_tens _ _)).
 apply dual_anti. intro v. apply tens_assocr. Qed.
+
+Lemma par_assoc_eq X Y Z : 
+  (par_sem X (par_sem Y Z)) = (par_sem (par_sem X Y) Z).
+Proof. apply iff_app_eq. split. apply par_assoc. apply par_assocr. Qed.
 
 (*
 Lemma ddp_comm X Y u : dual_sem (dual_sem (prods X Y)) u ->
@@ -507,9 +526,8 @@ sem of times redundant
 
 (* need to show correspondence between dual of formula and
   dual_sem (used in semantics definitions) *)
-Lemma sem_dual_fwd {V} sv A : (forall v, fact (sv v)) -> 
-  forall u, (sem sv (@dual V A) u) -> (dual_sem (sem sv A) u). 
-Proof. intros fsv. induction A ; simpl ; intros u.
+Lemma sem_dual_fwd A : forall u, (sem (@dual V A) u) -> (dual_sem (sem A) u). 
+Proof. induction A ; simpl ; intros u.
 - tauto.
 - apply dual_dual_sem.
 - apply dual_anti.  intro. rewrite dual_sem_1. tauto.
@@ -531,46 +549,44 @@ Proof. intros fsv. induction A ; simpl ; intros u.
 Print Implicit sub_dual_inv.
 Print Implicit prods_mono.
 
-Lemma sem_dual_bwd {V} sv A : (forall v, fact (sv v)) -> 
-  forall u, (dual_sem (sem sv A) u) -> (sem sv (@dual V A) u). 
-Proof. intros fsv. induction A ; simpl ; intros u.
+Lemma sem_dual_bwd A : forall u, (dual_sem (sem A) u) -> (sem (@dual V A) u). 
+Proof. induction A ; simpl ; intros u.
 - tauto.
-- exact (fsv v u).
+- apply fsv.
 - apply dual_anti. intro. rewrite dual_sem_1. tauto.
 - apply dual_anti. tauto.
 - rewrite ddd_iff. rewrite dual_sem_1. tauto.
 - tauto.
 - unfold par_sem. unfold tens_sem.  rewrite !ddd_iff.  apply dual_anti. 
-pose (dual_sub_inv (fact_sem _ _ fsv) IHA1) as dsd1.
-pose (dual_sub_inv (fact_sem _ _ fsv) IHA2) as dsd2.
+pose (dual_sub_inv (fact_sem _) IHA1) as dsd1.
+pose (dual_sub_inv (fact_sem _) IHA2) as dsd2.
 exact (prods_mono _ _ dsd1 dsd2).
 - apply dual_anti.  intro v. rewrite dual_sem_or.
-pose (dual_sub_inv (fact_sem _ _ fsv) IHA1) as dsd1.
-pose (dual_sub_inv (fact_sem _ _ fsv) IHA2) as dsd2.  firstorder.
+pose (dual_sub_inv (fact_sem _) IHA1) as dsd1.
+pose (dual_sub_inv (fact_sem _) IHA2) as dsd2.  firstorder.
 - unfold par_sem. unfold tens_sem.  rewrite ddd_iff.  apply dd_mono. 
 exact (prods_mono _ _ IHA1 IHA2).
 - rewrite ddd_iff. rewrite dual_sem_or. firstorder.
 - rewrite ddd_iff. apply dual_anti.
-pose (dual_sub_inv (fact_sem _ _ fsv) IHA) as dsd. firstorder.
+pose (dual_sub_inv (fact_sem _) IHA) as dsd. firstorder.
 - apply dd_mono. firstorder. Qed.
 
-Lemma sem_dual {V} sv A : (forall v, fact (sv v)) -> 
-  forall u, (sem sv (@dual V A) u) <-> (dual_sem (sem sv A) u).
-Proof. intros fsv u. split.
-apply (sem_dual_fwd _ _ fsv).  apply (sem_dual_bwd _ _ fsv). Qed.
+Lemma sem_dual A : forall u, (sem (@dual V A) u) <-> (dual_sem (sem A) u).
+Proof. intros u. split.
+apply (sem_dual_fwd _).  apply (sem_dual_bwd _). Qed.
 
 Print Implicit merge3LI.
 Print Implicit prodI.
 Print Implicit ds_ds_fact.
 
-Lemma sem_lolli {V} A B sv u : (forall v, fact (sv v)) ->
-  sem sv (@lolli V A B) u <-> lolli_sem (sem sv A) (sem sv B) u.
-Proof. intro fsv. unfold lolli. simpl. unfold par_sem.
+Lemma sem_lolli A B u :
+  sem (@lolli V A B) u <-> lolli_sem (sem A) (sem B) u.
+Proof. unfold lolli. simpl. unfold par_sem.
 rewrite curry_sem_bot_eqv.  unfold lolli_sem.
-pose (fun A => sem_dual _ A fsv).  clearbody i.  split.
+pose sem_dual.  clearbody i.  split.
 - intros dd * sa muvw. specialize (dd v w).  rewrite <- i in dd.
 rewrite dual_dual in dd.
-exact (fact_sem B sv fsv (dd sa muvw)).
+exact (fact_sem B (dd sa muvw)).
 - intros sabm * dda muvw.  rewrite <- i in dda. 
 rewrite dual_dual in dda. 
 exact (dual_dual_sem (sabm _ _ dda muvw)). Qed.
@@ -635,6 +651,60 @@ Definition par_sem_dual_eqv X Y fx fy u : iff _ _ :=
 Definition par_sem_eqv X Y fy u : iff _ _ :=
   conj (@par_sem_fwd' X Y u fy) (@par_sem_bwd X Y u). 
   
+Lemma par_sem_bot Y u : fact Y -> par_sem bot Y u -> Y u.
+Proof. intros fy pby.  apply (par_sem_fwd' fy) in pby. 
+exact (pby e u dual_sem_bot (cmrid cmM _)).  Qed.
+
+Lemma par_sem_botc Y u : fact Y -> par_sem Y bot u -> Y u.
+Proof. intros fy pby.  apply (par_sem_fwd' fact_bot) in pby. 
+exact (fy _ pby).  Qed.
+
+Lemma par_sem_botic Y u : fact Y -> Y u -> par_sem Y bot u.
+Proof. intros fy yu.  apply par_sem_bwd. eapply dd_mono.
+intros. exact H. exact (dual_dual_sem yu). Qed.
+
+Lemma par_sem_botc_eq Y : fact Y -> par_sem Y bot = Y.
+Proof. intro fy. apply iff_app_eq. intro x. split. 
+apply (par_sem_botc fy).  apply (par_sem_botic fy).  Qed.
+
+Definition par_sem_boti Y u fy yu := par_comm (@par_sem_botic Y u fy yu).
+
+Lemma seml_app' l l' : 
+  seml (l ++ l') = fold_right par_sem (seml l') (map sem l).
+Proof. unfold seml. rewrite map_app. apply fold_right_app. Qed.
+
+Lemma seml_app_lem l s : fact s -> 
+  fold_right par_sem s (map sem l) = par_sem (seml l) s.
+Proof. intro fs. induction l ; unfold seml ; simpl.
+- apply iff_app_eq.  intro x.  split.
+apply (par_sem_boti fs).  apply (par_sem_bot fs).
+- rewrite - par_assoc_eq.  apply f_equal. exact IHl. Qed.
+
+Lemma seml_app l l' : 
+  seml (l ++ l') = par_sem (seml l) (seml l').
+Proof. rewrite seml_app'.
+apply seml_app_lem. exact (fact_seml _).  Qed.
+
+Lemma seml_nil : seml [] = bot.  Proof. reflexivity. Qed.
+
+Lemma seml_cons A As : seml (A :: As) = par_sem (sem A) (seml As).
+Proof. reflexivity. Qed.
+
+Lemma seml_single A : seml [A] = sem A.
+Proof. unfold seml. simpl.
+apply par_sem_botc_eq. exact (fact_sem _). Qed.
+
+Lemma seml_merge xs ys zs :
+  merge xs ys zs -> seml zs = par_sem (seml xs) (seml ys).
+Proof. intro mrg. induction mrg.
+- rewrite !seml_cons. rewrite IHmrg. apply par_assoc_eq.
+- rewrite !seml_cons. rewrite IHmrg. rewrite !par_assoc_eq.
+  rewrite (par_comm_eq (sem y)). reflexivity.
+- unfold seml. simpl.  rewrite (par_sem_botc_eq fact_bot). reflexivity. Qed.
+
+Print Implicit par_sem_botc_eq.
+Print Implicit fact_sem.
+
 Lemma lolli_C (X Y Z : M -> Prop) u :
   lolli_sem X (lolli_sem Y Z) u -> lolli_sem Y (lolli_sem X Z) u.
 Proof. unfold lolli_sem.  intros xyz * yv me * xw mw.
@@ -672,64 +742,58 @@ Proof. apply par_sem_bwd. apply lolli_same_sound. Qed.
 Lemma id_sound X : par_sem (dual_sem X) X e.
 Proof. apply par_comm. apply id_sound'. Qed.
 
-Lemma one_sound V sv : sem sv (One V) e.
+Lemma one_sound : sem (One V) e.
 Proof. simpl. apply dual_dual_sem. reflexivity. Qed.
 
-Lemma top_ctxt_sound V sv X : par_sem X (sem sv (Top V)) e.
+Lemma top_ctxt_sound X : par_sem X (sem (Top V)) e.
 Proof. apply par_sem_bwd.  rewrite lolli_sem_e. simpl. tauto. Qed.
 
-Lemma bot_ctxt_sound V sv (X : M -> Prop) : 
-  X e -> par_sem X (sem sv (Bot V)) e.
+Lemma bot_ctxt_sound (X : M -> Prop) : 
+  X e -> par_sem X (sem (Bot V)) e.
 Proof. intro xe. apply par_sem_bwd.  rewrite lolli_sem_e. simpl.
 intro x. unfold dual_sem. unfold lolli_sem.
 intro xb.  exact (xb _ _ xe (cmrid cmM _)).  Qed.
 
 (* this should be true as par_sem is commutative, but
   similar proof fails, so par_sem_bwd must not be an equivalence
-Lemma bot_ctxt_sound' V sv (X : M -> Prop) : 
-  X e -> par_sem (sem sv (Bot V)) X e.
+Lemma bot_ctxt_sound' (X : M -> Prop) : 
+  X e -> par_sem (sem (Bot V)) X e.
   *)
 
-Lemma plusL_sem V sv A B u : sem sv A u -> sem sv (@plus V A B) u.
+Lemma plusL_sem A B u : sem A u -> sem (@plus V A B) u.
 Proof. intro sa. simpl. apply dual_dual_sem. exact (or_introl sa). Qed.
 
-Lemma plusL_ctxt_sound V sv (X : M -> Prop) A B u : 
-  par_sem X (sem sv A) u -> par_sem X (sem sv (@plus V A B)) u.
+Lemma plusL_ctxt_sound (X : M -> Prop) A B u : 
+  par_sem X (sem A) u -> par_sem X (sem (@plus V A B)) u.
 Proof. apply par_sem_mono. tauto. apply plusL_sem. Qed.
 
-Lemma plusR_sem V sv A B u : sem sv B u -> sem sv (@plus V A B) u.
+Lemma plusR_sem A B u : sem B u -> sem (@plus V A B) u.
 Proof. intro sa. simpl. apply dual_dual_sem. exact (or_intror sa). Qed.
 
-Lemma plusR_ctxt_sound V sv (X : M -> Prop) A B u : 
-  par_sem X (sem sv B) u -> par_sem X (sem sv (@plus V A B)) u.
+Lemma plusR_ctxt_sound (X : M -> Prop) A B u : 
+  par_sem X (sem B) u -> par_sem X (sem (@plus V A B)) u.
 Proof. apply par_sem_mono. tauto. apply plusR_sem. Qed.
 
-Lemma wth_ctxt_sound V sv (X : M -> Prop) A B u :
-  (forall v, fact (sv v)) -> par_sem X (sem sv A) u ->
-  par_sem X (sem sv B) u -> par_sem X (sem sv (@wth V A B)) u.
-Proof. intros fsv sa sb.
+Lemma wth_ctxt_sound (X : M -> Prop) A B u : par_sem X (sem A) u ->
+  par_sem X (sem B) u -> par_sem X (sem (@wth V A B)) u.
+Proof. intros sa sb.
 apply par_sem_bwd. unfold lolli_sem.
-pose (par_sem_fwd' (fact_sem _ _ fsv) sa) as la.
-pose (par_sem_fwd' (fact_sem _ _ fsv) sb) as lb.
+pose (par_sem_fwd' (fact_sem _) sa) as la.
+pose (par_sem_fwd' (fact_sem _) sb) as lb.
 unfold lolli_sem in la.  unfold lolli_sem in lb.
 intros * dxv muvw. simpl.  
 exact (conj (la v w dxv muvw) (lb v w dxv muvw)). Qed.
 
-Lemma tens_mrg_sound V sv X Y A B :
-  (forall v, fact (sv v)) -> par_sem X (sem sv A) e ->
-  par_sem Y (sem sv B) e -> par_sem (par_sem X Y) (sem sv (@tens V A B)) e.
-Proof. intros fsv sxa syb.
+Lemma tens_mrg_sound X Y A B : par_sem X (sem A) e ->
+  par_sem Y (sem B) e -> par_sem (par_sem X Y) (sem (@tens V A B)) e.
+Proof. intros sxa syb.
 apply par_sem_e_bwd.  intros v txy.
-pose (par_sem_fwd' (fact_sem _ _ fsv) sxa) as lxa.
-pose (par_sem_fwd' (fact_sem _ _ fsv) syb) as lyb.
+pose (par_sem_fwd' (fact_sem _) sxa) as lxa.
+pose (par_sem_fwd' (fact_sem _) syb) as lyb.
 unfold lolli_sem in lxa.  unfold lolli_sem in lyb.
 revert txy. apply tens_sem_mono ; intros u dsu.
 - exact (lxa u u dsu (cmlid cmM _)).
 - exact (lyb u u dsu (cmlid cmM _)).  Qed.
-
-Lemma par_sem_bot Y u : fact Y -> par_sem bot Y u -> Y u.
-Proof. intros fy pby.  apply (par_sem_fwd' fy) in pby. 
-exact (pby e u dual_sem_bot (cmrid cmM _)).  Qed.
 
 Hypothesis KsubJ : forall x, K x -> J x.
 Hypothesis Kidem : forall x, tens_sem K K x -> K x.
@@ -828,7 +892,7 @@ unfold dual_sem in dq.
 apply (ddK_e_lem fy ye).
 revert x dq. apply dd_mono. easy. Qed.
 
-(*
+(* this proof involves fact_K 
 Lemma wk_ctxt_sound (X Y : M -> Prop) : fact Y -> 
   Y e -> par_sem (query_sem X) Y e.
 Proof. intros fy ye.  apply par_sem_bwd'.
@@ -866,13 +930,84 @@ Print Implicit lolli_sem_e.
 Print Implicit dual_sub_inv.
 
 (* soundness of rules *)
-(* this might be difficult, need to prove inductively
-  that as par_sem is assoc and commutative, need to just use
-  par_sem context (principal formula) 
+Lemma merge_tens_sound ps c :
+  merge_ctxtg Tensrule ps c -> ForallT (fun p => seml p e) ps -> seml c e.
+Proof. intros m0 pss.
+destruct m0.  destruct m0.  inversion t. subst.
+rewrite !seml_app.
+rewrite (par_comm_eq _ (seml cr)).  apply par_assocr.
+rewrite seml_single.
+inversion pss. inversion H2. clear pss H2 H6. subst.
+rewrite seml_app in H1.  rewrite seml_app in H5.
+rewrite seml_cons in H1.  rewrite seml_cons in H5.
+rewrite (par_comm_eq (sem _)) in H1.
+rewrite (par_comm_eq (sem _)) in H5.
+rewrite par_assoc_eq in H5.  rewrite par_assoc_eq in H1.
+pose (tens_mrg_sound H1 H5). clearbody p. revert p.
+apply iffD1.  apply fun_cong.  apply fun_cong. apply f_equal.
+rewrite (seml_merge m0).  rewrite (seml_merge m1).
+rewrite !par_assoc_eq. apply fun_cong. apply f_equal.
+rewrite - !par_assoc_eq. apply f_equal. apply par_comm_eq. Qed.
+
+Lemma seml_fe Φ1 Φ2 As : seml (fmlsext Φ1 Φ2 As) e <->
+  (forall x : M, dual_sem (par_sem (seml Φ1) (seml Φ2)) x -> seml As x).
+Proof. unfold fmlsext. rewrite !seml_app.
+  rewrite - (par_comm_eq (seml Φ2)).  rewrite (par_assoc_eq).
+  rewrite (par_sem_eqv _ (fact_seml _) e). 
+  apply lolli_sem_e. Qed.
+
+Lemma llprinc_sound ps c :
+  fmlsruleg llprinc ps c -> ForallT (fun p => seml p e) ps -> seml c e.
+Proof. intros f pss. destruct f. destruct l.
+- (* Parrule *) destruct p. inversion pss. clear pss H2. subst.
+  revert H1. unfold fmlsext. rewrite !seml_app.
+  rewrite !seml_cons.  rewrite (par_assoc_eq (sem A)). easy.
+- (* Wthrule *) destruct w.  inversion pss. inversion H2.
+  clear pss H2 H6. subst. revert H1 H5.
+  rewrite !seml_fe. rewrite !seml_single. 
+  intros sa sb x dp.  exact (conj (sa x dp) (sb x dp)). 
+
+- (* PlusLrule *) destruct p. inversion pss. clear pss H2. subst.
+  revert H1.  rewrite !seml_fe. rewrite !seml_single. 
+  intros sa x dp.  pose (sa _ dp). simpl.
+  rewrite dual_sem_or'. clearbody s. revert s.
+  apply sub_dual_inv. easy.
+
+- (* PlusRrule *) destruct p. inversion pss. clear pss H2. subst.
+  revert H1.  rewrite !seml_fe. rewrite !seml_single. 
+  intros sa x dp.  pose (sa _ dp). simpl.
+  rewrite dual_sem_or'. clearbody s. revert s.
+  apply sub_dual_inv. easy.
+
+- (* Toprule *) destruct t.
+  rewrite !seml_fe. rewrite !seml_single. simpl. easy.
+
+- (* Botrule *) destruct b. inversion pss.  clear pss H2. subst.
+  revert H1. rewrite !seml_fe. rewrite seml_single. rewrite !seml_nil.
+  easy. Qed.
+
+Lemma mall_sound ps c :
+  @mall_rules V ps c -> ForallT (fun p => seml p e) ps -> seml c e.
+Proof. intros mpc pss.  destruct mpc.
+- (* llprinc *) exact (llprinc_sound f pss).
+- (* Tensrule *) exact (merge_tens_sound m0 pss).
+- (* Onerule *) destruct o. unfold seml. simpl.
+  apply par_sem_e_bwd. intro. rewrite dual_sem_eq_e. easy.
+- (* Id *) destruct i.  unfold seml. simpl.
+  apply par_sem_bwd. rewrite lolli_sem_e. 
+  intros. exact (par_sem_botic (@fact_dual _) H).
+- (* Idd *) destruct i.  unfold seml. simpl.
+  apply par_sem_bwd. rewrite lolli_sem_e.  intros.
+  apply (par_sem_botic (@fsv v)).  exact (@fsv v x H).
+Qed.
+
+Print Implicit par_sem_botic.
+Print Implicit eq_rect.
+
+(*
 Lemma maell_sound {V} sv ps c : (forall v, fact (sv v)) ->
   @maell_rules V ps c -> ForallT (fun p => seml sv p e) ps -> seml sv c e.
-Proof. intros fsv mpc pss.
-destruct mpc.
+Proof. intros fsv mpc pss.  destruct mpc.
 - (* mall_rules *) admit.
 - (* weakening *) destruct f. destruct w. sfs.
   unfold seml.
